gap proof
gap itself has index on the buffer

A B _ _ D E
0 1 2 3 4 5

gap left = 2
gap right = 3
gap length = gap right - gap left + 1

proof-isabelle-hol/GapBuffer.thy
@@ -2,6 +2,26 @@ theory GapBuffer
   imports Main   
 begin
 
+(* Invariant:
+
+   buffer = text before gap ++ gap ++ text after gap
+
+   gapLeft  = first gap cell
+   gapRight = last gap cell
+
+   The gap is the CLOSED interval [gapLeft, gapRight].
+
+   Valid indices satisfy
+
+      gapLeft \<le> gapRight
+      gapRight < length buffer
+
+   The logical contents of the editor are
+
+      take gapLeft buffer @ drop (gapRight + 1) buffer
+*)
+
+
 (* define a gap buffer datatype *)
 record GapBuffer =
   buffer   :: "char list"
@@ -9,18 +29,20 @@ record GapBuffer =
   gapRight :: "nat"
 
 
-(* what constitutes a valid buffer , gapLeft gapRight are natural numbers *)
-definition valid :: "GapBuffer \<Rightarrow> bool" where
-  "valid gb \<equiv>
-      gapLeft gb \<le> gapRight gb
-    \<and> gapRight gb \<le> length (buffer gb)"
 
 (* an empty buffer with 10 characters *)
 definition empty10 :: "GapBuffer" where
   "empty10 =
-     \<lparr> buffer = replicate 10 CHR ''x'',
+     \<lparr> buffer = replicate 10 CHR ''$'',
        gapLeft = 0,
        gapRight = 10 \<rparr>"
+
+definition empty3 :: "GapBuffer" where
+  "empty3 =
+     \<lparr> buffer = replicate 3 CHR ''$'',
+       gapLeft = 0,
+       gapRight = 3 \<rparr>"
+
 
 (* an empty buffer of size 0 with 0 characters - interesting ! *)
 definition empty0 :: "GapBuffer" where
@@ -39,7 +61,7 @@ value " CHR ''\<alpha>''  "
 (* an buffer of size 1 with 1 character capacity - also interesting ! *)
 definition empty1 :: "GapBuffer" where
   "empty1 =
-     \<lparr> buffer = [CHR ''\<alpha>''],
+     \<lparr> buffer = [CHR ''$''],
        gapLeft = 0,
        gapRight = 0 \<rparr>"
 
@@ -74,6 +96,7 @@ definition replace2 :: "char \<Rightarrow> nat \<Rightarrow> nat \<Rightarrow> c
                 else h # (replace2 c n (m+1) t))"
 *)
 
+(*
 (* given a char list if there exists index i with a character , replace it with this one  *)
 fun replace2 :: "char \<Rightarrow> nat \<Rightarrow> nat \<Rightarrow> char list \<Rightarrow> char list" where
   "replace2 c n m [] = []"
@@ -82,6 +105,30 @@ fun replace2 :: "char \<Rightarrow> nat \<Rightarrow> nat \<Rightarrow> char lis
 
 definition replace :: "char \<Rightarrow> nat \<Rightarrow> char list \<Rightarrow> char list" where
   "replace c n xs = replace2 c n 0 xs" 
+*)
+
+(*
+(* pedantic - replace returns Some xs if a replacement was actually made *)
+fun replace2 :: "char \<Rightarrow> nat \<Rightarrow> char list \<Rightarrow> char list" where
+  "replace2 c m [] = []"
+| "replace2 c 0 (h#t) = c # t"
+| "replace2 c (Suc n) (h#t) = h # (replace2 c n t)"
+
+fun replace :: "char \<Rightarrow> nat \<Rightarrow> char list \<Rightarrow> char list option" where
+  "replace c m xs = (if m \<ge> (length xs) then None else Some (replace2 c m xs))"
+
+(*unit tests for replace*)
+value " ''abc'' " (*abc*)
+value " replace (CHR ''d'') 0 ''abc'' "  (*Some dbc*)
+value " replace (CHR ''d'') 1 ''abc'' "  (*Some adc*)
+value " replace (CHR ''d'') 2 ''abc'' "  (*Some abd*)
+value " replace (CHR ''d'') 3 ''abc'' "  (*None rather than Some abc*)
+*)
+
+fun replace :: "char \<Rightarrow> nat \<Rightarrow> char list \<Rightarrow> char list" where
+  "replace c _ [] = []"
+| "replace c 0 (h # t) = c # t"
+| "replace c (Suc n) (h # t) = h # replace c n t"
 
 (*unit tests for replace*)
 value " ''abc'' " (*abc*)
@@ -100,10 +147,21 @@ fun lookup2 :: "nat \<Rightarrow> nat \<Rightarrow> char list \<Rightarrow> char
 definition lookup :: "nat \<Rightarrow> char list \<Rightarrow> char option" where
   "lookup n xs = lookup2 n 0 xs" 
 *)
-fun lookup :: "nat \<Rightarrow> char list \<Rightarrow> char option" where
-  "lookup m [] = None"
-| "lookup 0 (h#t) = Some h"
+
+(* its your responsibility to provide me with a valid natural number and list 
+if not then i am total and free to return anything *)
+fun lookup :: "nat \<Rightarrow> char list \<Rightarrow> char" where
+  "lookup m [] = CHR ''!''"
+| "lookup 0 (h#t) = h"
 | "lookup (Suc n) (h#t) = lookup n t"
+
+(*unit tests for lookup*)
+value " lookup 0 ''abc''"  (*a*)
+value " lookup 1 ''abc''"  (*b*)
+value " lookup 2 ''abc''"  (*c*)
+value " lookup 3 ''abc''"  (*!*)
+value " lookup 123 ''abc''"  (*!*)
+
 
 
 (* insert a character 
@@ -112,7 +170,7 @@ can insert a character if (gapRight gb) - (gapLeft gb) > 0
 *)
 definition insert :: "char \<Rightarrow> GapBuffer \<Rightarrow> GapBuffer" where
   "insert c gb =   
-   (if (gapRight gb) - (gapLeft gb) > 0 
+   (if (gapLeft gb) < (gapRight gb)  
     then
      gb\<lparr> buffer := replace c (gapLeft gb) (buffer gb),
          gapLeft := gapLeft gb + 1,
@@ -120,8 +178,12 @@ definition insert :: "char \<Rightarrow> GapBuffer \<Rightarrow> GapBuffer" wher
      else gb)"
 
 (*unit tests for insert*)
-value " insert (CHR ''a'') empty10 " (*axx...*)
-value " insert (CHR ''b'') (insert (CHR ''a'') empty10) " (*abxx...*)
+value " insert (CHR ''a'') empty3 " (*a//*)
+value " insert (CHR ''b'') (insert (CHR ''a'') empty3) " (*ab/*)
+value " insert (CHR ''c'') (insert (CHR ''b'') (insert (CHR ''a'') empty3)) " (*abc*)
+(* next one *abc* , notice how it does not include d  *)
+value " insert (CHR ''d'') 
+        (insert (CHR ''c'') (insert (CHR ''b'') (insert (CHR ''a'') empty3))) " 
 
 
 (* move a char list two hyphens ''  *)
@@ -148,6 +210,7 @@ value " List.hd ''abc'' "
 *)
 
 
+
 (* move left - note we needed parens around if..then..else 
  need to copy a character across 
  from (gapLeft gb) to (gapRight gb)
@@ -155,20 +218,76 @@ value " List.hd ''abc'' "
 definition move_left :: "GapBuffer \<Rightarrow> GapBuffer" where
   "move_left gb =
      (if gapLeft gb > 0 then     
-     gb\<lparr> gapLeft := gapLeft gb - 1,
+     let ch = lookup (gapLeft gb -1) (buffer gb)         
+     in let buf2 = replace ch (gapRight gb - 1) (buffer gb) 
+        in let buf3 = replace (CHR ''$'') (gapLeft gb - 1) buf2
+        in
+     gb\<lparr> buffer := buf3  ,
+         gapLeft := gapLeft gb - 1,
          gapRight := gapRight gb - 1 \<rparr>
      else gb)"
 
-(* move right - careful off by one error buffer is only as long as [length(buffer gb)-1] 
-although it says empty10 length 10 , it means list indices go from 0 .. 9 inclusive , 
- 10th indice is out of array bounds ! 
+
+
+(* *)
+definition abcd0 :: "GapBuffer" where
+  "abcd0 = insert (CHR ''d'') 
+           (insert (CHR ''c'') (insert (CHR ''b'') (insert (CHR ''a'') empty10)))"
+
+
+definition letfoo :: "int" where
+  "letfoo = (let a = 1 
+             in  a + 1 )" 
+
+definition letfoo2 :: "int" where
+  "letfoo2 = (let (a,b) = (1,2) 
+              in a + b)"
+
+value "letfoo" (*2*)
+value "letfoo2" (*3*)
+
+(* move right 
+
+let r be gapRight gb
+
+r \<ge> length buffer : no movement
+r < length buffer - movement 
+   if r = length buffer - 1 then r is the last valid index into ''array'' char list
+
+
 *)
 definition move_right :: "GapBuffer \<Rightarrow> GapBuffer" where
   "move_right gb =
-    (if gapRight gb > (length (buffer gb) - 1)
+    (if gapRight gb \<ge> length (buffer gb)
      then gb
-     else gb\<lparr> gapLeft := gapLeft gb + 1,
-         gapRight := gapRight gb + 1 \<rparr>)"
+     else let ch = lookup (gapRight gb) (buffer gb)         
+          in let buf2 = replace ch (gapLeft gb) (buffer gb)            
+          in let buf3 = replace (CHR ''$'') (gapRight gb) buf2 
+          in 
+          gb\<lparr> buffer := buf3 , 
+              gapLeft := gapLeft gb + 1,  
+              gapRight := gapRight gb + 1 \<rparr>)"
+
+
+
+
+value " abcd0 "
+value " move_left abcd0 "
+value " move_left (move_left abcd0) "
+value " move_left (move_left (move_left abcd0)) "
+value " move_left (move_left (move_left (move_left abcd0))) "
+value " move_right (move_left (move_left (move_left (move_left abcd0)))) "
+value " move_right (move_right ( move_left (move_left (move_left (move_left abcd0))))) "
+value " move_right (move_right (move_right ( move_left (move_left (move_left (move_left abcd0)))))) "
+value " move_right (move_right (move_right (move_right ( move_left (move_left (move_left (move_left abcd0))))))) "
+value " move_left (move_right (move_right (move_right (move_right ( move_left (move_left (move_left (move_left abcd0)))))))) "
+value " move_left (move_left (move_right (move_right (move_right (move_right ( move_left (move_left (move_left (move_left abcd0))))))))) "
+value " move_left (move_left (move_left (move_right (move_right (move_right (move_right ( move_left (move_left (move_left (move_left abcd0)))))))))) "
+value " move_left (move_left (move_left (move_left (move_right (move_right (move_right (move_right ( move_left (move_left (move_left (move_left abcd0))))))))))) "
+
+value " replace (CHR ''y'') 3 ''abcdxxxxxx'' "
+
+
 
 (*move_right unit tests - expect no movement on an empty buffer 
 also useful for move_left as it has same semantics *)
@@ -196,16 +315,112 @@ value "insert (CHR ''d'') (move_left (insert (CHR ''c'')
 (* delete a character *)
 definition delete_char :: "GapBuffer \<Rightarrow> GapBuffer" where
   "delete_char gb =
-     gb\<lparr> gapLeft := gapLeft gb + 1,
-         gapRight := gapRight gb + 1 \<rparr>"
+     (if gapLeft gb = 0 then gb 
+     else let buf = replace (CHR ''$'') (gapLeft gb - 1) (buffer gb)
+          in gb\<lparr> buffer := buf, 
+                 gapLeft := gapLeft gb - 1,
+                 gapRight := gapRight gb + 1 \<rparr>)"
 
-(* move to a specific index - combination of move left or right as required *)
-(**)
+(*delete unit tests*)
+value "delete_char empty10" 
+value "delete_char (delete_char empty10)"
+value "delete_char (delete_char (delete_char empty10))"
+value "abcd0"
+value "delete_char abcd0" (*abc///...*)
+value "delete_char (delete_char abcd0)" (*ab///...*)
+value "delete_char (delete_char (delete_char abcd0))" (*a///...*)
+value "delete_char (delete_char (delete_char (delete_char abcd0)))" (*///...*)
+value "delete_char (delete_char (delete_char (delete_char (delete_char abcd0))))" (*///...*)
+
+(* small buffer of length 3 - simple tests *)
+
+value " insert (CHR ''d'') 
+        (insert (CHR ''c'') (insert (CHR ''b'') (insert (CHR ''a'') empty3))) " 
+(* abc  *)
+
+value " delete_char (insert (CHR ''d'') 
+        (insert (CHR ''c'') (insert (CHR ''b'') (insert (CHR ''a'') empty3)))) " 
+(* ab/  *)
+
+value " delete_char (delete_char (insert (CHR ''d'') 
+        (insert (CHR ''c'') (insert (CHR ''b'') (insert (CHR ''a'') empty3))))) " 
+(* a//  *)
+
+value " delete_char(delete_char (delete_char (insert (CHR ''d'') 
+        (insert (CHR ''c'') (insert (CHR ''b'') (insert (CHR ''a'') empty3)))))) " 
+(* ///  *)
+
+
+
+value " ''abc'' @ ''def'' " (*abcdef*)
+value " take 2 ''abcdef'' " (*ab*)
+value " drop 2 ''abcdef'' " (*cdef*)
+value " (take 2 ''abcdef'') @ (take 2 ''abcdef'')" (*abab*)
+value " let x =(take 2 ''abcdef'') in x @ x " (*abab*)
+value " let s = ''abcdef'' in
+        let x = take 2 s in
+        let y = drop 2 s in
+           y @ x " (*cdefab*)
+
+
+definition contents :: "GapBuffer \<Rightarrow> char list" where
+  "contents gb = (let buf = buffer gb in
+                 let before = take (gapLeft gb) buf in 
+                 let after  = drop (gapRight gb) buf in 
+                 before @ after)"
+
+(*contents unit tests - as we move left the gap splits the text into before and after 
+check visually that contents preserves the text and ignores the gap 
+*)
+
+value "abcd0" (*abcd///...*)
+
+value "contents abcd0" (*abcd*)
+value "contents empty10" (*[]*)
+
+value "(move_left abcd0)" (*abc////d*)
+value "contents (move_left abcd0)" (*abcd*)
+
+value "(move_left (move_left abcd0))" (*ab////cd*)
+value "contents (move_left (move_left abcd0))" (*abcd*)
+
+value "(move_left (move_left (move_left abcd0)))" (*a///bcd*)
+value "contents (move_left (move_left (move_left abcd0)))" (*abcd*)
+
+value "(move_left (move_left (move_left (move_left abcd0))))" (*////abcd*)
+value "contents (move_left (move_left (move_left (move_left abcd0))))" (*abcd*)
+
+
+(* what constitutes a valid buffer , gapLeft gapRight are natural numbers *)
+definition valid :: "GapBuffer \<Rightarrow> bool" where
+  "valid gb \<equiv>
+      gapLeft gb \<le> gapRight gb
+    \<and> gapRight gb \<le> length (buffer gb)"
+
+definition garb1 :: "GapBuffer" where
+  "garb1 =
+     \<lparr> buffer = [CHR ''$''],
+       gapLeft = 1,
+       gapRight = 1 \<rparr>"
+
+value "garb1" 
+value "valid garb1" 
+value "garb1" 
+value "move_left garb1"
+value "insert (CHR ''b'') (move_left garb1)"
+value "move_right garb1"
+value "move_left (move_right garb1)"
+value "move_left (move_left (move_right garb1))"
+value "move_right (move_left (move_left (move_right garb1)))"
+value "insert (CHR ''b'') (move_right (move_left (move_left (move_right garb1))))"
+value "delete_char (move_right (move_left (move_left (move_right garb1))))"
+
+lemma contents_move_left:
+  "valid gb \<Longrightarrow> contents (move_left gb) = contents gb"
+proof
+  by auto
+qed
 
 
 
 
-
-
-
- 
